\documentclass{beamer}
\title{Two proofs in the margin}
\author{Bharathi Ramana Joshi}
\begin{document}
\maketitle
\begin{frame}
    \frametitle{Infinite descent}
    Proof by contradiction\\
    Idea: Proposition $P(x_1,x_2,\dots)$
\end{frame}

\begin{frame}
    \frametitle{Fermat's Last Theorem}
    \begin{gather*}
        a^n+b^n=c^n
    \end{gather*}
    \begin{enumerate}
        \item $a,b,c\in\mathbb{Z}^+$
        \item $n\in\mathbb{Z}^+,n>2$
    \end{enumerate}
\end{frame}

\begin{frame}
    \frametitle{Fermat's Last Theorem, $n = 4$}
    \begin{gather}
        a^4+b^4=c^4\\
        a^4+b^4=c^2
    \end{gather}
\end{frame}

\begin{frame}
    \frametitle{Fermat's Last Theorem, $n = 4$}
    \framesubtitle{$a^4+b^4=c^2$}
    \begin{enumerate}
        \item Coprime
        \item Both $a$ and $b$ not even
        \item Both $a$ and $b$ not odd ($\because odd^4\equiv 1 \mod 4$)
    \end{enumerate}
\end{frame}

\begin{frame}
    \frametitle{Fermat's Last Theorem, $n = 4$}
    \framesubtitle{$a^4+b^4=c^2$}
    \begin{enumerate}
        \item Coprime
        \item Both $a$ and $b$ not even
        \item Both $a$ and $b$ not odd ($\because odd^4\equiv 1 \mod 4$)
        \item Only possible case : one even and one odd
    \end{enumerate}
\end{frame}

\begin{frame}
    \frametitle{Fermat's Last Theorem, $n = 4$}
    \framesubtitle{a even, b odd}
    \begin{gather*}
        (a^2)^2 + (b^2)^2 = c^2
    \end{gather*}

    Thus $(a^2, b^2, c)$ primitive Pythagorean triplet,

    \begin{gather}
        a^2 = 2mn\\
        b^2 = m^2 - n^2\\
        c = m^2 + n^2
    \end{gather}
\end{frame}

\begin{frame}
    \frametitle{Pythagorean triplet}
    \framesubtitle{$m^2 = b^2 + n^2$}
    $b$ odd $\implies n$ even
    \begin{gather}
        n = 2xy\\
        b = x^2 - y^2\\
        m = x^2 + y^2
    \end{gather}
\end{frame}

\begin{frame}
    \frametitle{Coprimes}
    \framesubtitle{Equation 1 : $a^2=2mn$\\Equation 6 : $n = 2xy$}
    \begin{gather}
        m(n/2) = (a/2)^2
    \end{gather}
    Thus both $m$ and $n/2$ squares. From 6,
    \begin{gather}
        xy = n/2
    \end{gather}
    Thus both $x$ and $y$ squares.\\
    Put
    \begin{gather}
        x = u^2\\
        y = v^2\\
        m = w^2
    \end{gather}
\end{frame}

\begin{frame}
    \frametitle{Descent}
    \framesubtitle{Equation 8 : $m = x^2+ y^2$}
    From 8,
    \begin{gather}
        m = x^2+y^2\\
        \implies w^2 = u^4 + v^4
    \end{gather}
\end{frame}

\begin{frame}
    \frametitle{Alternate proof}
    \framesubtitle{a even, b odd\\ Equation 2 : $a^4+b^4=c^2$}
    Rewriting 2,
    \begin{gather}
        a^4 = c^2 - b^4 = (c - b^2)(c + b^2)
    \end{gather}
    Observations
    \begin{enumerate}
        \item No odd prime divides both
        \item Both even (since $a$ even and $b$ odd)
        \item 4 does not divide both
    \end{enumerate}
    Therefore, gcd$(c-b^2, c+b^2)$ = 2\\
\end{frame}

\begin{frame}
    \frametitle{Alternate proof}
    \framesubtitle{$a^4 = (c - b^2)(c + b^2)$}
    Either case \# 1:
    \begin{gather}
        c - b^2 = 2x^4(x > 0 \textrm{ (odd)})\\
        c + b^2 = 8y^4, gcd(x, y) = 1
    \end{gather}
    or case \# 2:
    \begin{align}
        c - b^2 &= 8y^4\\
        c + b^2 &= 2x^4,(x > 0 \textrm{ (odd)}, gcd(x, y) = 1)
    \end{align}
\end{frame}

\begin{frame}
    \frametitle{Alternate proof}
    \framesubtitle{Case \# 1}
    \begin{align}
        c + b^2 &= 8y^4, gcd(x, y) = 1\\
        c - b^2 &= 2x^4(x > 0 \textrm{ (odd)})
    \end{align}
    impossible, since
    \begin{gather*}
        (c + b^2) - (c - b^2) = 2b^2 = -2x^4 + 8y^4\\
        \implies x^2\equiv -1\mod 4
    \end{gather*}
\end{frame}

\begin{frame}
    \frametitle{Alternate proof}
    \framesubtitle{Descent}
    Case \#2
    \begin{align}
        c + b^2 &= 2x^4,(x > 0 \textrm{ (odd)}, (x, y) = 1)\\
        c - b^2 &= 8y^4
    \end{align}
    \begin{gather*}
        b^2 = x^4 - 4y^4\implies 4y^4 = (x^2+b)(x^2-b)
    \end{gather*}
    By similar argument $gcd(x^2+b, x^2-b) = 2$. Therefore
    \begin{align}
        x^2-b &= 2u^4\\
        x^2+b &= 2v^4\\
        \implies x^2 &= u^4 + v^4
    \end{align}
\end{frame}

\begin{frame}
    \frametitle{Summary}
    Show that if one solution exists, smaller solution exists leading to
    impossible infinite chain
\end{frame}

\end{document}
